inlining: cexp proof finished, only termination cheated

compiler/backend/passes/proofs/pure_inline_cexpProofScript.sml
@@ -2,7 +2,14 @@
   Inlining optimization proofs for cexp
 *)
 open HolKernel Parse boolLib bossLib BasicProvers;
-open listTheory pairTheory topological_sortTheory;
+open fixedPointTheory arithmeticTheory listTheory stringTheory alistTheory
+     optionTheory pairTheory ltreeTheory llistTheory bagTheory dep_rewrite
+     BasicProvers pred_setTheory relationTheory rich_listTheory finite_mapTheory
+     combinTheory mlmapTheory indexedListsTheory;
+open pure_expTheory pure_valueTheory pure_evalTheory pure_eval_lemmasTheory
+     pure_exp_lemmasTheory pure_limitTheory pure_exp_relTheory
+     pure_alpha_equivTheory pure_miscTheory pure_congruenceTheory
+     pure_letrec_seqTheory pure_demandTheory;
 open pure_cexpTheory pure_varsTheory balanced_mapTheory pureLangTheory;
 open pure_inlineTheory pure_inline_cexpTheory;
 
@@ -15,22 +22,665 @@ End
 
 (* xs and m have the same elements *)
 Definition memory_inv_def:
-  memory_inv xs m =
-    ∀v e. (MEM (explode v, (crhs_to_rhs e)) xs) ⇔ (lookup m v = SOME e)
+  memory_inv xs m ⇔
+    { explode a | ∃e. lookup m a = SOME e } = set (MAP FST xs) ∧
+    ∀v e. (lookup m v = SOME e) ⇒ (MEM (explode v, (crhs_to_rhs e)) xs)
 End
 
-(* check assumptions *)
-Theorem inline_cexp_list_subst_rel:
-  ∀h m x xs.
-    memory_inv xs m ∧
-    no_shadowing (exp_of x) ∧
-    DISJOINT (set (MAP FST xs)) (boundvars (exp_of x)) ⇒
-    list_subst_rel xs (exp_of x) (exp_of (inline m h x))
+Theorem inline_list_empty:
+  (inline_list m ns h l = ([], ns1)) ⇒ l = []
 Proof
-  \\ cheat
-  (* evantually: ho_match_mp_tac *)
+  rw []
+  \\ Cases_on `l`
+  >- fs []
+  \\ fs [inline_def]
+  \\ Cases_on `inline m ns h h'`
+  \\ gvs []
+  \\ Cases_on `inline_list m r h t`
+  \\ gvs []
 QED
 
+Theorem no_shadowing_Apps_EVERY:
+  ∀e es.
+    no_shadowing (Apps e es) ⇒
+    no_shadowing e ∧ EVERY no_shadowing es
+Proof
+  strip_tac
+  \\ Induct_on `es` using SNOC_INDUCT
+  >- fs [Apps_def]
+  \\ fs [Apps_def,SNOC,Apps_SNOC,EVERY_SNOC]
+QED
+
+Theorem no_shadowing_Letrec_EVERY:
+  ∀e xs.
+    no_shadowing (Letrec xs e) ⇒
+      no_shadowing e ∧
+      EVERY (λ(v, e). no_shadowing e) xs ∧
+      DISJOINT (boundvars e) (set (MAP FST xs))
+Proof
+  strip_tac
+  \\ strip_tac
+  \\ simp [Once no_shadowing_cases]
+  \\ strip_tac
+  \\ fs [DISJOINT_SYM,EVERY_MEM]
+  \\ rw []
+  \\ Cases_on `e'`
+  \\ last_x_assum $ qspec_then `(q,r)` assume_tac
+  \\ gvs []
+QED
+
+Theorem list_subst_rel_Apps:
+  (∀ts us l t1 u1.
+    list_subst_rel l t1 u1 ∧
+    LIST_REL (list_subst_rel l) ts us ⇒
+    list_subst_rel l (Apps t1 ts) (Apps u1 us))
+Proof
+  Induct
+  >- fs [Apps_def]
+  \\ fs [Apps_def,PULL_EXISTS]
+  \\ rw []
+  \\ last_x_assum irule
+  \\ fs []
+  \\ irule list_subst_rel_App
+  \\ fs []
+QED
+
+Theorem memory_inv_APPEND:
+  memory_inv xs m ∧
+  map_ok m ∧
+  ¬MEM (explode v) (MAP FST xs) ⇒
+  memory_inv (xs ++ [(explode v,Exp (exp_of e1))]) (insert m v (cExp e1))
+Proof
+  gvs [memory_inv_def]
+  \\ rw []
+  >- (
+    fs [EXTENSION,mlmapTheory.lookup_insert,AllCaseEqs()]
+    \\ metis_tac []
+  )
+  \\ gvs [mlmapTheory.lookup_insert,AllCaseEqs()]
+  \\ gvs [crhs_to_rhs_def,exp_of_def]
+QED
+
+Theorem memory_inv_APPEND_Rec:
+  memory_inv xs m ∧
+  map_ok m ∧
+  ¬MEM (explode v) (MAP FST xs) ⇒
+  memory_inv (xs ++ [(explode v,Rec (exp_of e1))]) (insert m v (cRec e1))
+Proof
+  gvs [memory_inv_def]
+  \\ rw []
+  >- (
+    fs [EXTENSION,mlmapTheory.lookup_insert,AllCaseEqs()]
+    \\ metis_tac []
+  )
+  \\ gvs [mlmapTheory.lookup_insert,AllCaseEqs()]
+  \\ gvs [crhs_to_rhs_def,exp_of_def]
+QED
+
+Theorem DISJOINT_boundvars_Apps:
+  ∀s e es.
+    DISJOINT (boundvars (Apps e es)) s ⇒
+    DISJOINT (boundvars e) s ∧
+    EVERY (λx. DISJOINT (boundvars x) s) es
+Proof
+  strip_tac
+  \\ strip_tac
+  \\ Induct using SNOC_INDUCT
+  >- fs [Apps_def]
+  \\ fs [Apps_def,SNOC,Apps_SNOC]
+  \\ strip_tac
+  \\ strip_tac
+  \\ simp [boundvars_def]
+  \\ gvs []
+  \\ fs [EVERY_SNOC]
+QED
+
+Theorem EVERY_DISJOINT_MEM:
+  ∀s xs.
+    (∀s1. MEM s1 xs ⇒ DISJOINT s1 s) ⇒
+    EVERY (λx. DISJOINT x s) xs
+Proof
+  rw []
+  \\ simp [EVERY_MEM]
+QED
+
+Theorem SND_intro:
+  (λ(p1, p2). p2) = SND
+Proof
+  simp [FUN_EQ_THM,FORALL_PROD]
+QED
+
+Theorem branch_vars_eq_lemma:
+  ∀bs cs.
+    LENGTH bs = LENGTH cs ⇒
+    MAP (λx. FST (SND x)) (MAP2 (λ(v,vs,_) e. (v,vs,e)) bs cs) =
+      MAP (λx. FST (SND x)) bs
+Proof
+  Induct_on `bs`
+  >- fs []
+  \\ Cases_on `h`
+  \\ Cases_on `r`
+  \\ Cases_on `cs`
+  >- fs [FST,SND,MAP2]
+  \\ fs [FST,SND,MAP2]
+QED
+
+Theorem inline_list_size_EQ:
+  ∀l l1 ns.
+    inline_list m ns h l = (l1, ns1) ⇒
+      LENGTH l = LENGTH l1
+Proof
+  Induct_on `l`
+  >- fs [inline_def]
+  \\ rw [inline_def]
+  \\ Cases_on `inline m ns h h'`
+  \\ gvs []
+  \\ Cases_on `inline_list m r h l`
+  \\ gvs []
+  \\ last_x_assum irule
+  \\ gvs []
+  \\ qexists `r`
+  \\ gvs []
+QED
+
+Theorem list_subst_rel_lets_for:
+  list_subst_rel xs a b ⇒
+  list_subst_rel xs
+    (lets_for c v vs a)
+    (lets_for c v vs b)
+Proof
+  rw []
+  \\ Induct_on `vs`
+  >- fs [lets_for_def]
+  \\ rw []
+  \\ Cases_on `h`
+  \\ fs [lets_for_def]
+  \\ irule list_subst_rel_App
+  \\ irule_at Any list_subst_rel_Lam
+  \\ fs [list_subst_rel_refl]
+QED
+
+Theorem lets_for_no_shadowing:
+  ∀vs a.
+    no_shadowing (lets_for c v vs a) ⇒
+    no_shadowing a
+Proof
+  strip_tac
+  \\ Induct_on `vs`
+  >- fs [lets_for_def]
+  \\ rw []
+  \\ Cases_on `h`
+  \\ fs [lets_for_def]
+QED
+
+Theorem lets_for_DISJOINT:
+  ∀vs a s.
+    DISJOINT (boundvars (lets_for c v vs a)) s ⇒
+    DISJOINT (boundvars a) s
+Proof
+  strip_tac
+  \\ Induct_on `vs`
+  >- fs [lets_for_def]
+  \\ rw []
+  \\ Cases_on `h`
+  \\ fs [lets_for_def]
+QED
+
+val lemma = inline_ind
+  |> Q.SPEC `λm ns h x. ∀xs t ns1.
+    memory_inv xs m ∧
+    map_ok m ∧
+    no_shadowing (exp_of x) ∧
+    DISJOINT (set (MAP FST xs)) (boundvars (exp_of x)) ∧
+    (inline m ns h x) = (t, ns1) ⇒
+    list_subst_rel xs (exp_of x) (exp_of t)`
+  |> Q.SPEC `λm ns h es. ∀xs ts ns1.
+    memory_inv xs m ∧
+    map_ok m ∧
+    EVERY (λe. no_shadowing (exp_of e)) es ∧
+    EVERY (λx. DISJOINT (set (MAP FST xs)) (boundvars (exp_of x))) es ∧
+    (inline_list m ns h es) = (ts, ns1) ⇒
+    LIST_REL (λx t. list_subst_rel xs (exp_of x) (exp_of t)) es ts`
+  |> SIMP_RULE std_ss []
+
+Theorem inline_cexp_list_subst_rel:
+  ^(lemma |> concl |> rand)
+Proof
+  match_mp_tac lemma
+  \\ rpt strip_tac
+  >~ [`Var _ _`] >- (
+    Cases_on `inline m ns h (Var a v) = (Var a v, _)`
+    >- gvs [list_subst_rel_refl,exp_of_def]
+    \\ gvs [inline_def]
+    \\ Cases_on `lookup m v` \\ gvs [list_subst_rel_refl]
+    \\ Cases_on `x` \\ gvs [list_subst_rel_refl]
+    \\ Cases_on `is_Lam c` \\ gvs [memory_inv_def,list_subst_rel_refl,exp_of_def]
+    \\ irule list_subst_rel_VarSimp
+    \\ res_tac
+    \\ fs [crhs_to_rhs_def]
+  )
+  >~ [`Prim _ _ _`] >- (
+    gvs [inline_def]
+    \\ Cases_on `inline_list m ns h es`
+    \\ gvs []
+    \\ gvs [memory_inv_def,list_subst_rel_refl,exp_of_def,FORALL_PROD]
+    \\ irule list_subst_rel_Prim
+    \\ fs [LIST_REL_MAP,o_DEF,FORALL_PROD,LIST_REL_MAP2,PULL_EXISTS]
+    \\ last_x_assum irule
+    \\ fs []
+    \\ fs [EVERY_MAP]
+    \\ simp [EVERY_MEM]
+    \\ rw []
+    \\ first_x_assum $ qspec_then `boundvars (exp_of x)` assume_tac
+    \\ fs [MAP_MAP_o,o_DEF]
+    \\ first_x_assum irule
+    \\ fs [MEM_MAP]
+    \\ rw []
+    \\ qexists `x`
+    \\ rw []
+  )
+  >~ [`App _ _ _`] >- (
+    gvs [inline_def]
+    \\ Cases_on `inline m ns h e`
+    \\ gvs []
+    \\ Cases_on `inline_list m r h es`
+    \\ gvs []
+    \\ rename [`list_subst_rel _ _ (exp_of (App a t ts))`]
+    \\ gvs [exp_of_def,SF ETA_ss]
+    \\ irule list_subst_rel_Apps
+    \\ fs [LIST_REL_MAP,o_DEF]
+    \\ last_x_assum $ irule_at Any
+    \\ last_x_assum $ irule_at Any
+    \\ gvs [memory_inv_def,DISJOINT_SYM]
+    \\ qspecl_then [`set (MAP FST xs)`,`exp_of e`,`MAP exp_of es`] assume_tac DISJOINT_boundvars_Apps
+    \\ drule no_shadowing_Apps_EVERY
+    \\ strip_tac
+    \\ fs [EVERY_MAP,DISJOINT_SYM]
+  )
+  >~ [`Lam _ _`] >- (
+    gvs [inline_def]
+    \\ Cases_on `inline m ns h e`
+    \\ gvs []
+    \\ gvs [memory_inv_def,list_subst_rel_refl,exp_of_def,FORALL_PROD]
+    \\ Induct_on `vs`
+    >- fs [Lams_def,list_subst_rel_refl,inline_def,exp_of_def,MAP]
+    \\ rw []
+    \\ gvs [Lams_def]
+    \\ irule list_subst_rel_Lam
+    \\ last_x_assum irule
+  )
+  >~ [`Let _ _ _`] >- (
+    gvs [inline_def]
+    \\ Cases_on `inline m ns h e1`
+    \\ gvs []
+    \\ Cases_on `inline (heuristic_insert m h v e1) r h e2`
+    \\ gvs []
+    \\ gvs [list_subst_rel_refl,exp_of_def]
+    \\ fs [heuristic_insert_def]
+    \\ Cases_on `h e1`
+    >- (
+      irule list_subst_rel_Let
+      \\ conj_tac
+      >- (
+        last_x_assum irule
+        \\ fs [DISJOINT_SYM,memory_inv_def]
+      )
+      \\ last_x_assum irule
+      \\ fs [DISJOINT_SYM]
+      \\ fs [mlmapTheory.insert_thm]
+      \\ irule memory_inv_APPEND
+      \\ fs []
+    )
+    \\ fs []
+    \\ irule list_subst_rel_App
+    \\ reverse $ conj_tac
+    >- (
+      last_x_assum irule
+      \\ fs [DISJOINT_SYM,memory_inv_def]
+    )
+    \\ irule list_subst_rel_Lam
+    \\ last_x_assum irule
+    \\ fs [DISJOINT_SYM,memory_inv_def]
+  )
+  >~ [`Letrec _ _ _`] >- (
+    gvs [inline_def]
+    \\ Cases_on `inline_list m ns h (MAP SND vbs)`
+    \\ gvs []
+    \\ Cases_on `inline (heuristic_insert_Rec m h vbs) r h e`
+    \\ gvs []
+    \\ gvs [list_subst_rel_refl,exp_of_def]
+    \\ Cases_on `heuristic_insert_Rec m h vbs = m`
+    >- (
+      irule list_subst_rel_Letrec
+      \\ last_x_assum $ irule_at Any
+      \\ gvs []
+      \\ drule no_shadowing_Letrec_EVERY
+      \\ strip_tac \\ fs [DISJOINT_SYM]
+      \\ gvs [MAP_MAP_o,o_DEF,FORALL_PROD,LAMBDA_PROD,SND_intro,EVERY_MAP]
+      \\ last_x_assum $ qspec_then `xs` assume_tac
+      \\ sg `EVERY (λ(p1,p2). DISJOINT (boundvars (exp_of p2)) (set (MAP FST xs))) vbs`
+      >- (
+        simp [EVERY_MEM]
+        \\ rw []
+        \\ Cases_on `e'`
+        \\ gvs []
+        \\ first_x_assum $ qspec_then `boundvars (exp_of r')` assume_tac
+        \\ first_x_assum irule
+        \\ gvs [MEM_MAP]
+        \\ qexists `(q'',r')`
+        \\ gvs []
+      )
+      \\ last_x_assum drule
+      \\ pop_assum mp_tac
+      \\ pop_assum mp_tac
+      \\ qpat_x_assum `DISJOINT _ _` mp_tac
+      \\ qid_spec_tac `q`
+      \\ qid_spec_tac `vbs`
+      \\ Induct
+      >- fs []
+      \\ fs [PULL_EXISTS,FORALL_PROD]
+    )
+    \\ gvs [heuristic_insert_Rec_def]
+    \\ Cases_on `vbs`
+    >- gvs []
+    \\ reverse $ Cases_on `t`
+    >- gvs []
+    \\ PairCases_on `h'`
+    \\ rename [`(w, u)`]
+    \\ gvs []
+    \\ Cases_on `¬h u`
+    >- gvs []
+    \\ gvs []
+    \\ Cases_on `q`
+    >- (
+      gvs [MAP2,inline_def]
+      \\ Cases_on `inline m ns h u`
+      \\ gvs []
+    )
+    \\ reverse $ Cases_on `t`
+    >- (
+      gvs [MAP2,inline_def]
+      \\ Cases_on `inline m ns h u`
+      \\ gvs []
+    )
+    \\ gvs [MAP2,inline_def]
+    \\ irule list_subst_rel_LetrecIntro
+    \\ last_x_assum $ irule_at Any
+    \\ fs [DISJOINT_SYM]
+    \\ fs [mlmapTheory.insert_thm]
+    \\ irule_at Any memory_inv_APPEND_Rec
+    \\ fs []
+    \\ drule no_shadowing_Letrec_EVERY
+    \\ rw []
+  )
+  >~ [`Case _ _ _ _ _`] >- (
+    gvs [inline_def]
+    \\ Cases_on `inline m ns h e`
+    \\ gvs []
+    \\ Cases_on `inline_list m r h (MAP (λ(v, vs, e). e) bs)`
+    \\ gvs []
+    \\ Cases_on `(case f of
+        NONE => (NONE,r')
+      | SOME (vs,e') =>
+        (λ(e4,ns4). (SOME (vs,e4),ns4)) (inline m r' h e'))`
+    \\ gvs []
+    \\ sg `LENGTH (MAP (λ(v,vs,e). e) bs) = LENGTH q'`
+    >- (
+      irule inline_list_size_EQ
+      \\ metis_tac []
+    )
+    \\ fs [LENGTH_MAP]
+    \\ sg `MAP (λx. FST (SND x)) (MAP2 (λ(v,vs,_) e. (v,vs,e)) bs q') =
+      MAP (λx. FST (SND x)) bs`
+    >- (
+      irule branch_vars_eq_lemma
+      \\ gvs []
+    )
+    \\ gvs [memory_inv_def,list_subst_rel_refl,exp_of_def,o_DEF]
+    \\ gvs [MAP_MAP_o,o_DEF,FST,SND,MAP_ZIP,FST_intro]
+    \\ sg `f = NONE ⇔ q'' = NONE`
+    >- (
+      Cases_on `f`
+      >- fs []
+      \\ PairCases_on `x`
+      \\ gvs []
+      \\ Cases_on `inline m r' h x1`
+      \\ gvs []
+    )
+    \\ sg `(∀v1 x1. f = SOME (v1, x1) ⇒ no_shadowing (exp_of x1))`
+    >- (
+      rw []
+      \\ Cases_on `MEM v (FLAT (MAP (λx. FST (SND x)) bs))`
+      >- (
+        gvs []
+        \\ qpat_x_assum `no_shadowing (rows_of _ _ _)` mp_tac
+        \\ qid_spec_tac `bs`
+        \\ Induct
+        >- fs [rows_of_def,IfDisj_def]
+        \\ rw []
+        \\ Cases_on `h'`
+        \\ Cases_on `r''`
+        \\ fs [rows_of_def,IfDisj_def,MAP]
+      )
+      \\ gvs []
+      \\ qpat_x_assum `no_shadowing (rows_of _ _ _)` mp_tac
+      \\ qid_spec_tac `bs`
+      \\ Induct
+      >- fs [rows_of_def,IfDisj_def]
+      \\ rw []
+      \\ Cases_on `h'`
+      \\ Cases_on `r''`
+      \\ fs [rows_of_def,IfDisj_def,MAP]
+    )
+    \\ sg `EVERY (λe. no_shadowing (exp_of e)) (MAP (λ(v,vs,e). e) bs)`
+    >- (
+      rw []
+      \\ Cases_on `MEM v (FLAT (MAP (λx. FST (SND x)) bs))`
+      >- (
+        gvs []
+        \\ qpat_x_assum `no_shadowing (rows_of _ _ _)` mp_tac
+        \\ qid_spec_tac `bs`
+        \\ Induct
+        >- fs [rows_of_def,IfDisj_def]
+        \\ rw []
+        \\ Cases_on `h'`
+        \\ Cases_on `r''`
+        \\ fs [rows_of_def,lets_for_def,IfDisj_def,MAP,MAPi_def]
+        \\ irule lets_for_no_shadowing
+        \\ metis_tac []
+      )
+      \\ gvs []
+      \\ qpat_x_assum `no_shadowing (rows_of _ _ _)` mp_tac
+      \\ qid_spec_tac `bs`
+      \\ Induct
+      >- fs [rows_of_def,IfDisj_def]
+      \\ rw []
+      \\ Cases_on `h'`
+      \\ Cases_on `r''`
+      \\ fs [rows_of_def,lets_for_def,IfDisj_def,MAP,MAPi_def]
+      \\ irule lets_for_no_shadowing
+      \\ metis_tac []
+    )
+    \\ sg `(∀v1 x1. f = SOME (v1, x1) ⇒ DISJOINT (boundvars (exp_of x1)) (set (MAP FST xs)))`
+    >- (
+      rw []
+      \\ Cases_on `MEM v (FLAT (MAP (λx. FST (SND x)) bs))`
+      >- (
+        gvs []
+        \\ qpat_x_assum `DISJOINT (boundvars (rows_of _ _ _)) (set (MAP FST xs))` mp_tac
+        \\ qid_spec_tac `bs`
+        \\ Induct
+        >- fs [rows_of_def,IfDisj_def]
+        \\ rw []
+        \\ Cases_on `h'`
+        \\ Cases_on `r''`
+        \\ fs [rows_of_def,lets_for_def,IfDisj_def,MAP,MAPi_def]
+      )
+      \\ gvs []
+      \\ qpat_x_assum `DISJOINT (boundvars (rows_of _ _ _)) (set (MAP FST xs))` mp_tac
+      \\ qid_spec_tac `bs`
+      \\ Induct
+      >- fs [rows_of_def,IfDisj_def]
+      \\ rw []
+      \\ Cases_on `h'`
+      \\ Cases_on `r''`
+      \\ fs [rows_of_def,lets_for_def,IfDisj_def,MAP,MAPi_def]
+    )
+    \\ sg `EVERY (λx. DISJOINT (boundvars (exp_of x)) (set (MAP FST xs))) (MAP (λ(v,vs,e). e) bs)`
+    >- (
+      rw []
+      \\ Cases_on `MEM v (FLAT (MAP (λx. FST (SND x)) bs))`
+      >- (
+        gvs []
+        \\ qpat_x_assum `DISJOINT (boundvars (rows_of _ _ _)) (set (MAP FST xs))` mp_tac
+        \\ qid_spec_tac `bs`
+        \\ Induct
+        >- fs [rows_of_def,IfDisj_def]
+        \\ rw []
+        \\ Cases_on `h'`
+        \\ Cases_on `r''`
+        \\ fs [rows_of_def,lets_for_def,IfDisj_def,MAP,MAPi_def]
+        \\ irule lets_for_DISJOINT
+        \\ metis_tac []
+      )
+      \\ gvs []
+      \\ qpat_x_assum `DISJOINT (boundvars (rows_of _ _ _)) (set (MAP FST xs))` mp_tac
+      \\ qid_spec_tac `bs`
+      \\ Induct
+      >- fs [rows_of_def,IfDisj_def]
+      \\ rw []
+      \\ Cases_on `h'`
+      \\ Cases_on `r''`
+      \\ fs [rows_of_def,lets_for_def,IfDisj_def,MAP,MAPi_def]
+      \\ irule lets_for_DISJOINT
+      \\ metis_tac []
+    )
+    \\ sg `list_subst_rel xs
+      (rows_of (explode v)
+          (case f of NONE => Fail | SOME (a,e) => IfDisj v a (exp_of e))
+          (MAP (λ(c,vs,x'). (explode c,MAP explode vs,exp_of x')) bs))
+      (rows_of (explode v)
+          (case q'' of NONE => Fail | SOME (a,e) => IfDisj v a (exp_of e))
+          (MAP (λ(c,vs,x'). (explode c,MAP explode vs,exp_of x'))
+            (MAP2 (λ(v,vs,_) e. (v,vs,e)) bs q')))`
+    >- (
+      last_x_assum $ qspec_then `xs` assume_tac
+      \\ pop_assum mp_tac
+      \\ pop_assum mp_tac
+      \\ pop_assum mp_tac
+      \\ pop_assum mp_tac
+      \\ pop_assum mp_tac
+      \\ pop_assum mp_tac
+      \\ pop_assum mp_tac
+      \\ qpat_x_assum `inline_list m r h (MAP (λ(v,vs,e). e) bs) = (q',r')` mp_tac
+      \\ qid_spec_tac `r`
+      \\ qid_spec_tac `q'`
+      \\ qid_spec_tac `bs`
+      \\ Induct
+      >- (
+        rw []
+        \\ fs [rows_of_def,MAP2]
+        \\ Cases_on `f`
+        >- fs [list_subst_rel_refl]
+        \\ PairCases_on `x`
+        \\ gvs []
+        \\ Cases_on `q''`
+        >- fs []
+        \\ PairCases_on `x`
+        \\ Cases_on `inline m r' h x1`
+        \\ gvs [IfDisj_def]
+        \\ irule list_subst_rel_Prim
+        \\ fs [LIST_REL_EL_EQN,list_subst_rel_refl]
+        \\ last_x_assum irule
+        \\ fs [DISJOINT_SYM]
+      )
+      \\ rpt strip_tac
+      \\ fs [rows_of_def,MAP2,MAP]
+      \\ Cases_on `h'`
+      \\ rename [`(a,b)::bs`]
+      \\ Cases_on `b`
+      \\ rename [`MAP2 _ _ qs`]
+      \\ Cases_on `qs`
+      >- fs []
+      \\ gvs [rows_of_def,MAP2,MAP,FORALL_PROD]
+      \\ irule list_subst_rel_Prim
+      \\ simp [LIST_REL_EL_EQN,list_subst_rel_refl,lets_for_def]
+      \\ irule_at Any list_subst_rel_lets_for
+      \\ gvs [DISJOINT_SYM]
+      \\ rename [`inline_list m r h (head::MAP (λ(v,vs,e). e) bs)`]
+      \\ gvs [DISJOINT_SYM,memory_inv_def,inline_def]
+      \\ Cases_on `inline m r h head`
+      \\ gvs []
+      \\ rename [`inline_list m r1 h (MAP (λ(v,vs,e). e) bs)`]
+      \\ Cases_on `inline_list m r1 h (MAP (λ(v,vs,e). e) bs)`
+      \\ gvs []
+      \\ first_x_assum $ irule_at Any
+      \\ gvs []
+      \\ metis_tac []
+    )
+    \\ Cases_on `MEM v (FLAT (MAP (λx. FST (SND x)) bs))`
+    >- (
+      gvs []
+      \\ irule list_subst_rel_Prim
+      \\ fs [LIST_REL_def,list_subst_rel_refl]
+      \\ irule list_subst_rel_App
+      \\ first_x_assum $ irule_at Any
+      \\ fs [DISJOINT_SYM,memory_inv_def]
+      \\ irule list_subst_rel_Lam
+      \\ fs []
+    )
+    \\ gvs []
+    \\ irule list_subst_rel_App
+    \\ first_x_assum $ irule_at Any
+    \\ fs [DISJOINT_SYM,memory_inv_def]
+    \\ irule list_subst_rel_Lam
+    \\ fs []
+  )
+  >~ [`NestedCase _ _ _ _ _ _`] >- (
+    gvs [inline_def,list_subst_rel_refl]
+  )
+  >~ [`LIST_REL _ [] _`] >- (
+    gvs [inline_def]
+  )
+  \\ gvs [inline_def]
+  \\ Cases_on `inline m ns h e`
+  \\ gvs []
+  \\ Cases_on `inline_list m r h es`
+  \\ gvs []
+QED
+
+Theorem inline_cexp_list_subst_rel_spec:
+  ∀m ns h x xs t ns1.
+    memory_inv xs m ∧
+    map_ok m ∧
+    no_shadowing (exp_of x) ∧
+    DISJOINT (set (MAP FST xs)) (boundvars (exp_of x)) ∧
+    (inline m ns h x) = (t, ns1) ⇒
+    list_subst_rel xs (exp_of x) (exp_of t)
+Proof
+  rw []
+  \\ assume_tac inline_cexp_list_subst_rel
+  \\ gvs []
+  \\ last_x_assum irule
+  \\ gvs []
+  \\ metis_tac []
+QED
+
+Theorem inline_all_thm:
+  ∀h x.
+    no_shadowing (exp_of x) ∧
+    closed (exp_of x) ∧
+    (t, ns1) = inline_all h x ⇒
+    (exp_of x) ≅ (exp_of t)
+Proof
+  rw []
+  \\ irule list_subst_rel_IMP_exp_eq
+  \\ fs [inline_all_def]
+  \\ irule inline_cexp_list_subst_rel_spec
+  \\ fs []
+  \\ qexists `h` \\ qexists `empty` \\ qexists `empty` \\ qexists `ns1`
+  \\ fs [map_ok_empty,memory_inv_def] 
+QED
 
 (*******************)
 
