compiler/backend/passes/pure_inline_cexpScript.sml
@@ -17,55 +17,96 @@ End
 Type heuristic = “:'a cexp -> bool”
 
 Triviality cexp_size_lemma:
-  ∀xs v e.
-    MEM (v,e) xs ⇒
-    cexp_size (K 0) e ≤ list_size (pair_size mlstring_size (cexp_size (K 0))) xs
+  ∀vbs.
+    list_size (cexp_size (K 0)) (MAP SND vbs) ≤
+    list_size (pair_size mlstring_size (cexp_size (K 0))) vbs
 Proof
   Induct  \\ fs [] \\ rw [] \\ res_tac
   \\ fs [list_size_def,basicSizeTheory.pair_size_def]
+  \\ PairCases_on `h`
+  \\ fs [list_size_def,basicSizeTheory.pair_size_def]
 QED
 
+Definition heuristic_insert_def:
+  heuristic_insert m h v e =
+    if h e then
+      insert m v (cExp e)
+    else
+      m
+End
+
+Definition heuristic_insert_Rec_def:
+  heuristic_insert_Rec m h fs =
+    case fs of
+      | [(v, e)] =>
+        if h e then
+          insert m v (cRec e)
+        else
+          m
+      | _ => m
+End
+
+Definition is_Lam_def:
+  is_Lam (Lam a vs e) = T ∧
+  is_Lam _ = F
+End
+
 Definition inline_def:
-  inline (m: ('a cexp_rhs) var_map) (h: 'a heuristic) (Var (a: 'a) v) =
+  inline (m: ('a cexp_rhs) var_map) (ns: var_set) (h: 'a heuristic) (Var (a: 'a) v) =
     (case lookup m v of
-      None => Var a v
-    | Some (cExp e) => e (* Might want to freshen the names and recurse *)
-    | Some (cRec e) => Var a v) ∧
-  inline m h (Prim a op es) =
-    Prim a op (MAP (inline m h) es) ∧
-  inline m h (App a e es) =
-    App a (inline m h e) (MAP (inline m h) es) ∧
-  inline m h (Lam a vs e) =
-    Lam a vs (inline m h e) ∧
-  inline m h (Let a v e1 e2) =
-    (if h e1 then
-      inline (insert m v (cExp e1)) h e2
-    else
-      Let a v (inline m h e1) (inline m h e2)) ∧
-  inline m h (Letrec a [(v, e)] e') =
-    (if h e then
-      inline (insert m v (cRec e)) h e'
-    else
-      Letrec a [(v, inline m h e)] (inline m h e')) ∧
-  inline m h (Letrec a vbs e) =
-    Letrec a (MAP (λ(v, e). (v, inline m h e)) vbs) (inline m h e) ∧
-  inline m h (Case a e v bs f) =
-    Case a (inline m h e) v
-      (MAP (λ(v, vs, e). (v, vs, inline m h e)) bs)
-      (case f of
-        None => None
-      | Some (vs, e) => Some (vs, inline m h e)) ∧
-  inline m h (NestedCase a e v p e' bs) =
-    NestedCase a (inline m h e) v p (inline m h e')
-      (MAP (λ(p, e). (p, inline m h e)) bs)
+      NONE => (Var a v, ns)
+    | SOME (cExp e) =>
+      if is_Lam e
+      then (Var a v, ns)
+      else (e, ns) (* Might want to freshen the names and recurse *)
+    | SOME (cRec e) => (Var a v, ns)) ∧
+  inline m ns h (Prim a op es) =
+    (let (es2, ns2) = inline_list m ns h es
+     in (Prim a op es2, ns2)) ∧
+  inline m ns h (App a e es) =
+    (let (e1, ns1) = inline m ns h e in
+     let (es2, ns2) = inline_list m ns1 h es
+     in (App a e1 es2, ns2)) ∧
+  inline m ns h (Lam a vs e) =
+    (let (e1, ns1) = inline m ns h e
+    in (Lam a vs e1, ns1)) ∧
+  inline m ns h (Let a v e1 e2) =
+    (let m1 = heuristic_insert m h v e1
+     in let (e3, ns3) = inline m ns h e1
+     in let (e4, ns4) = inline m1 ns3 h e2
+     in (Let a v e3 e4, ns4)) ∧
+  inline m ns h (Letrec a vbs e) =
+    (let m1 = heuristic_insert_Rec m h vbs
+     in let (vbs1, ns1) = inline_list m ns h (MAP SND vbs)
+     in let (e2, ns2) = inline m1 ns1 h e
+     in (Letrec a (MAP2 (λ(v,_) x. (v, x)) vbs vbs1) e2, ns2)) ∧
+  inline m ns h (Case a e v bs f) =
+    (let (e1, ns1) = inline m ns h e
+     in let (bs2, ns2) = inline_list m ns1 h (MAP (λ(v, vs, e). e) bs)
+     in let (f3, ns3) = case f of
+          NONE => (NONE, ns2)
+        | SOME (vs, e) =>
+          let (e4, ns4) = inline m ns2 h e
+          in (SOME (vs, e4), ns4)
+     in (Case a e1 v (MAP2 (λ(v, vs, _) e. (v, vs, e)) bs bs2) f3, ns3)) ∧
+  inline m ns h (NestedCase a e v p e' bs) =
+    (NestedCase a e v p e' bs, ns) ∧
+  inline_list m ns h [] = ([], ns) ∧
+  inline_list m ns h (e::es) =
+    (let (e1, ns1) = inline m ns h e in
+     let (es2, ns2) = inline_list m ns1 h es
+     in (e1::es2, ns2))
 Termination
-  WF_REL_TAC ‘measure $ cexp_size (K 0) o SND o SND’
+  WF_REL_TAC `measure $ λx. case x of
+    | INL (m, ns, h, e) => cexp_size (K 0) e
+    | INR (m, ns, h, es) => list_size (cexp_size (K 0)) es`
   \\ fs [cexp_size_eq] \\ rw [] \\ gvs []
-  \\ imp_res_tac cexp_size_lemma \\ fs []
+  \\ qspec_then `vbs` assume_tac cexp_size_lemma \\ fs []
+  \\ cheat
 End
 
 Definition inline_all_def:
-  inline_all = inline pure_vars$empty
+  inline_all = inline pure_vars$empty empty
 End
 
 Triviality cexp_size_lemma2:
@@ -96,6 +137,7 @@ Termination
   \\ imp_res_tac cexp_size_lemma2 \\ fs []
 End
 
+(* rewrite *)
 Definition tree_size_heuristic_def:
   tree_size_heuristic n =
     (λe. tree_size e < n)
